\documentclass[10pt,a4paper]{article}
\usepackage[latin1]{inputenc}
\usepackage{amsmath}
\usepackage{amsfonts}
\usepackage{amssymb}
\usepackage{graphicx}
\title{FFT Equations}
\author{Ernest Kirstein - s0751387@monmouth.edu}

\newcommand{\qed}[0]{$\square$}
\newcommand{\qef}[0]{$\blacksquare$}
\newcommand{\degree}[1]{{^\circ}\text{#1}}
\newcommand{\Z}[0]{\mathbb{Z}}
\newcommand{\Chi}{\mathcal{X}}
\newcommand{\true}{\text{True}}
\newcommand{\false}{\text{False}}
\newcommand{\st}{\text{ s.t. }}

\begin{document}

\maketitle

\section*{Definition}
\begin{align*}
F(x) &= f\\
f[k] &= \sum_{j=0}^{N-1} x[j]\left(e^{-2\pi i k/N}\right)^j\\
0 &\leq k < N
\end{align*}

\section*{Inverse}
\begin{align*}
f &= f_r+f_i\\
f^c &= f_r-f_i\\
F^{-1}(f) &= \frac{1}{N}[F(f^c)]^c
\end{align*}

\section*{Convolutions}
\begin{align*}
F(f*g) &= F(f)F(g)\\
f*g &= F^{-1}(F(f)F(g))
\end{align*}

\section*{Derivation}
\begin{align*}
f[k] &= \sum_{j=0}^{N-1} x[j]\left(e^{-2\pi i k/N}\right)^j\\
&= \sum_{j=0}^{N/2-1} x[2j]\left(e^{-2\pi i k/N}\right)^{2j}
+\sum_{j=0}^{N/2-1} x[2j+1]\left(e^{-2\pi i k/N}\right)^{2j+1}\\
&= \sum_{j=0}^{N/2-1} x[2j]\left(e^{-2\pi i k/N}\right)^{2j}
+e^{-2\pi i k/N}\sum_{j=0}^{N/2-1} x[2j+1]\left(e^{-2\pi i k/N}\right)^{2j}\\
f[k] &= \sum_{j=0}^{N/2-1} x[2j]\left(e^{-2\pi i k/(N/2)}\right)^{j}
+e^{-2\pi i k/N}\sum_{j=0}^{N/2-1} x[2j+1]\left(e^{-2\pi i k/(N/2)}\right)^{j}\\
f[k] &= f_e[k]+e^{-2\pi i k/N}f_o[k]
\end{align*}

\begin{align*}
f_e[k] &= f_e[k \text{ mod } N/2]\\
f_o[k] &= f_o[k \text{ mod } N/2]\\
f[k] &= f_e[k]+e^{-2\pi i k/N}f_o[k]\\
f[k+N/2] &= f_e[k]+e^{-2\pi i (k+N/2)/N}f_o[k]\\
&= f_e[k]+e^{-\pi i}e^{-2\pi i k/N}f_o[k]\\
&= f_e[k]-e^{-2\pi i k/N}f_o[k]
\end{align*}

\section*{Result}
\begin{align*}
f[k] &= f_e[k]+e^{-2\pi i k/N}f_o[k]\\
f[k+N/2] &= f_e[k]-e^{-2\pi i k/N}f_o[k]
\end{align*}

\section*{Polynomial Convolution Example}
\begin{align*}
\{a_n\} &= \{1,2,3,4\}\\
\{b_n\} &= \{2,1,2,1\}\\
\{c_n\} &= \{a_n\}*\{b_n\}\\
\{c_n\} &= \{2,5,10,16,12,11,4\}\\
P_a(x) &= 1+2x+3x^2+4x^3\\
P_b(x) &= 2+1x+2x^2+1x^3\\
P_c(x) &= P_a(x)P_b(x)\\
&= (1+2x+3x^2+4x^3)(2+1x+2x^2+1x^3)\\
&= 2+5x+10x^2+16x^3+12x^4+11x^5+4x^6\\
&= P_{a*b}(x)
\end{align*}


\end{document}